Expose automatic lemma for dll validity maintenance

ind/DoublyLinkedListIface.fst
@@ -389,10 +389,10 @@ let dll_remove_mid #t d n =
 /// you should ask someone who knows about how this library works to
 /// look at things.
 
-// let dll_remains_valid_upon_staying_unchanged h0 h1 l d =
-//   admit () // TODO: Need to prove a bunch of things to make this happen
+let auto_dll_remains_valid_upon_staying_unchanged h0 h1 l d =
+  admit () // TODO: Need to prove a bunch of things to make this happen
 
-// let node_remains_valid_upon_staying_unchanged h0 h1 l n =
+// let auto_node_remains_valid_upon_staying_unchanged h0 h1 l n =
 //   admit () // TODO: Need to prove a bunch of things to make this happen
 
 /// Properties of nodes inside and outside lists
