ind/DoublyLinkedListIface.fsti
@@ -253,15 +253,15 @@ val dll_remove_mid (#t:Type0) (d:dll t) (n:node t) :
 /// you should ask someone who knows about how this library works to
 /// look at things.
 
-// val dll_remains_valid_upon_staying_unchanged (h0 h1:HS.mem) (l:B.loc) (d:dll 'a) :
-//   Lemma
-//     (requires (dll_valid h0 d /\
-//                B.modifies l h0 h1 /\
-//                B.loc_disjoint (fp_dll h0 d) l))
-//     (ensures (dll_valid h1 d))
-//     [SMTPat (dll_valid h0 d); SMTPat (dll_valid h1 d); SMTPat (B.loc_disjoint (fp_dll h0 d) l)]
+val auto_dll_remains_valid_upon_staying_unchanged (h0 h1:HS.mem) (l:B.loc) (d:dll 'a) :
+  Lemma
+    (requires (dll_valid h0 d /\
+               B.modifies l h0 h1 /\
+               B.loc_disjoint (fp_dll h0 d) l))
+    (ensures (dll_valid h1 d))
+    [SMTPat (dll_valid h0 d); SMTPat (dll_valid h1 d); SMTPat (B.modifies l h0 h1)]
 
-// val node_remains_valid_upon_staying_unchanged (h0 h1:HS.mem) (l:B.loc) (n:node 'a) :
+// val auto_node_remains_valid_upon_staying_unchanged (h0 h1:HS.mem) (l:B.loc) (n:node 'a) :
 //   Lemma
 //     (requires (node_valid h0 n /\
 //                B.modifies l h0 h1 /\
