ind/Example.fst
@@ -10,7 +10,6 @@ let main () : HST.Stack unit (fun _ -> True) (fun _ _ _ -> True) =
   let d : DLL.dll UInt32.t = DLL.dll_new () in
   let n = DLL.node_of 1ul in
   let h0 = HST.get () in
-  assume (DLL.dll_valid h0 d);
   assume (DLL.fp_node n `B.loc_disjoint` DLL.fp_dll h0 d);
   DLL.dll_insert_at_head d n;
   HST.pop_frame ()
